src/Vellvm/typings_props.v
@@ -1,6 +1,7 @@
 Add LoadPath "./ott".
 Add LoadPath "./monads".
 Add LoadPath "./compcert".
+Add LoadPath "./GraphBasics".
 Add LoadPath "../../../theory/metatheory_8.3".
 Require Import syntax.
 Require Import infrastructure.
@@ -179,6 +180,16 @@ Proof.
       subst. auto.
 Qed.
 
+Lemma wf_fdef__blockInFdefB__wf_block : forall b ifs S M f,
+  blockInFdefB b f = true -> 
+  wf_fdef ifs S M f ->
+  wf_block ifs S M f b.
+Proof.
+  intros.
+  inv H0.  
+  eapply wf_blocks__wf_block; eauto.
+Qed.
+
 Lemma wf_system__blockInFdefB__wf_block : forall b f ps los nts s ifs,
   blockInFdefB b f = true -> 
   InProductsB (product_fdef f) ps = true ->
@@ -262,6 +273,33 @@ Proof.
   inv H1. auto.
 Qed.
 
+Lemma wf_fdef__wf_cmd : forall l1 ps1 cs1 tmn1 ifs s m f c,
+  blockInFdefB (block_intro l1 ps1 cs1 tmn1) f = true -> 
+  wf_fdef ifs s m f ->
+  In c cs1 ->
+  wf_insn ifs s m f (block_intro l1 ps1 cs1 tmn1) (insn_cmd c).
+Proof.
+  intros.
+  eapply wf_fdef__blockInFdefB__wf_block in H; eauto.
+  inv H. eapply wf_cmds__wf_cmd; eauto.
+Qed.
+
+Lemma wf_fdef__wf_tmn : forall l1 ps1 cs1 tmn1 ifs s m f,
+  blockInFdefB (block_intro l1 ps1 cs1 tmn1) f = true -> 
+  wf_fdef ifs s m f ->
+  wf_insn ifs s m f (block_intro l1 ps1 cs1 tmn1) (insn_terminator tmn1).
+Proof.
+  intros.
+  eapply wf_fdef__blockInFdefB__wf_block in H; eauto.
+  inv H. auto.
+Qed.
+
+Lemma wf_fdef__non_entry: forall ifs s m f, 
+  wf_fdef ifs s m f -> getEntryBlock f <> None.
+Proof.
+  intros. inv H. rewrite H5. congruence.
+Qed.
+
 Lemma wf_tmn__wf_value : forall ifs s m f b tmn v,
   wf_insn ifs s m f b (insn_terminator tmn) ->
   valueInTmnOperands v tmn ->
@@ -333,7 +371,6 @@ Qed.
 Lemma wf_phi_operands__elim : forall f b i0 t0 vls0 vid1 l1 n,
   wf_phi_operands f b i0 t0 vls0 ->
   nth_list_value_l n vls0 = Some (value_id vid1, l1) ->
-  (vid1 <> i0 \/ (not (isReachableFromEntry f b))) /\
   exists vb, exists b1,
     lookupBlockViaIDFromFdef f vid1 = Some vb /\
     lookupBlockViaLabelFromFdef f l1 = Some b1 /\
@@ -341,12 +378,7 @@ Lemma wf_phi_operands__elim : forall f b i0 t0 vls0 vid1 l1 n,
 Proof.
   induction vls0; intros.
     destruct n; inversion H0.
-
-    destruct v; inv H.
-      destruct n; inv H0; eauto.
-        split; auto.        
-        exists vb. exists b1. split; auto.
-      destruct n; inv H0; eauto.
+    destruct v; inv H; destruct n; inv H0; eauto.
 Qed.
 
 Lemma wf_value_list__getValueViaLabelFromValuels__wf_value : forall
@@ -602,7 +634,6 @@ Proof.
                 (transfer (bound_blocks bs)) ((le, start) :: nil)) as R1.
     destruct start.
     destruct bs_contents; tinv Hp.
-    destruct bs_contents; tinv Hp.
     destruct R1; subst.
     SCase "analysis is done".
       symmetry in HeqR1.
@@ -645,14 +676,14 @@ Proof.
       subst.
       unfold Dominators.top in Heqdefs3, Heqdefs'.
       simpl in Heqdefs3, Heqdefs'.
+      destruct bs; tinv HeqR.
+      destruct b; inv HeqR.
       assert (exists ps, exists cs, exists tmn,
-        getEntryBlock (fdef_intro fh bs) = Some (block_intro a ps cs tmn)).
-        unfold entry_dom in HeqR.
-        destruct bs.
-          inversion HeqR.
-          destruct b. inv HeqR.
-          exists p. exists c. exists t. auto.
-      assert (l' <> a) as Neq.
+        getEntryBlock (fdef_intro fh ((block_intro l0 p c t) :: bs)) = 
+          Some (block_intro l0 ps cs tmn)) as H.
+        unfold entry_dom in HeqR1.
+        exists p. exists c. exists t. auto.
+      assert (l' <> l0) as Neq.
         clear - H Hsucc HwfF HBinF. 
         destruct H as [ps1 [cs1 [tmn1 H]]].
         eapply getEntryBlock_inv; eauto.
@@ -665,6 +696,1715 @@ Proof.
   Case "entry is wrong".   
     subst. inversion HBinF.
 Qed.
+
+Lemma wf_tmn__in_successors: forall ifs s m f l0 cs ps tmn l1
+  (HuniqF : uniqFdef f)
+  (Hwftmn : wf_insn ifs s m f (block_intro l0 cs ps tmn) (insn_terminator tmn))
+  (Hin : In l1 (successors_terminator tmn)),
+  exists cs1, exists ps1, exists tmn1, 
+    blockInFdefB (block_intro l1 cs1 ps1 tmn1) f.
+Proof.
+  intros.
+  inv Hwftmn; simpl in Hin; tinv Hin.
+    destruct Hin as [Hin | [Hin | Hin]]; tinv Hin; subst.
+      destruct block1.
+      apply lookupBlockViaLabelFromFdef_inv in H2; auto.
+      destruct H2 as [J1 J2]; subst; eauto.
+
+      destruct block2.
+      apply lookupBlockViaLabelFromFdef_inv in H3; auto.
+      destruct H3 as [J1 J2]; subst; eauto.
+
+    destruct Hin as [Hin | Hin]; tinv Hin; subst.
+      apply lookupBlockViaLabelFromFdef_inv in H0; auto.
+      destruct H0 as [J1 J2]; subst; eauto.
+Qed.
+
+Require Import Dipaths.
+
+Module DomComplete. Section DomComplete.
+  
+Variable ifs : intrinsic_funs.
+Variable S : system.
+Variable M : module.
+Variable fh : fheader.
+Variable bs : blocks.
+Definition bound := bound_blocks bs.
+Definition predecessors := make_predecessors (successors_blocks bs).
+Definition transf := transfer bound.
+Definition top := Dominators.top bound.
+Definition bot := Dominators.bot bound.
+Definition dt := DomDS.dt bound.
+Variable entry: l.
+Variable entrypoints: list (atom * dt).
+
+Hypothesis wf_entrypoints:
+  predecessors!!!entry = nil /\
+  match bs with
+  | block_intro l0 _ _ _ :: _ => l0 = entry
+  | _ => False 
+  end /\
+  exists v, [(entry, v)] = entrypoints /\ Dominators.eq _ v top.
+
+Hypothesis HwfF: wf_fdef ifs S M (fdef_intro fh bs).
+Hypothesis HuniqF: uniqFdef (fdef_intro fh bs).
+
+Definition non_sdomination (l1 l2:l) : Prop :=
+  let vertexes := vertexes_fdef (fdef_intro fh bs) in
+  let arcs := arcs_fdef (fdef_intro fh bs) in
+  exists vl, exists al, 
+    D_walk vertexes arcs (index l2) (index entry) vl al /\
+    ~ In (index l1) vl.
+
+Definition non_sdomination_prop (res: AMap.t dt) : Prop :=
+  forall l1 l2, 
+    vertexes_fdef (fdef_intro fh bs) (index l1) ->
+    ~ Dominators.member _ l1 res!!l2 -> 
+    non_sdomination l1 l2.
+    
+Lemma start_non_sdomination: 
+  non_sdomination_prop 
+    (DomDS.st_in _ (DomDS.start_state _ (successors_blocks bs) entrypoints)).
+Proof.
+  intros l1 l2 Hin Hnotin.
+  destruct (eq_atom_dec l2 entry); try subst l2.
+    unfold non_sdomination.
+    exists V_nil. exists A_nil. 
+    split. 
+      constructor.
+      destruct wf_entrypoints as [_ [J _]].
+      destruct bs; tinv J.
+      destruct b; subst.
+      eapply entry_in_vertexes; simpl; eauto.
+
+      intro J. inv J.
+
+    eapply EntryDomsOthers.dom_nonentry_start_state_in in n; eauto.
+    contradict Hnotin.
+    unfold DomDS.start_state. simpl.
+    apply Dominators.member_eq with (x2:=bot); auto.
+Qed.
+
+Lemma non_sdomination_refl : forall l1,
+  l1 <> entry ->
+  reachable (fdef_intro fh bs) l1 ->
+  non_sdomination l1 l1.
+Proof.
+  unfold reachable, non_sdomination.
+  intros.  
+  destruct bs; simpl in *.
+    inv H0.
+    destruct b; simpl in *.
+    destruct H0 as [vl [al H0]].
+    apply DWalk_to_dpath in H0.
+    destruct H0 as [vl0 [al0 Hp]].
+    exists vl0. exists al0. 
+    destruct wf_entrypoints as [_ [Heq _]]; subst.
+    split.
+      apply D_path_isa_walk; auto.
+      eapply DP_endx_ninV; eauto. congruence.
+Qed.
+
+Lemma propagate_succ_non_sdomination: forall st p n out
+  (Hinpds: In p predecessors!!!n)
+  (Hout: Dominators.ge _ (transf p st.(DomDS.st_in _)!!p) out)
+  (Hdom: non_sdomination_prop st.(DomDS.st_in _)),
+  non_sdomination_prop (DomDS.propagate_succ _ st out n).(DomDS.st_in _).
+Proof.
+  unfold non_sdomination_prop. intros.
+  destruct (@DomDS.propagate_succ_spec _ st out n) as [J1 J2].
+  destruct (eq_atom_dec n l2) as [Heq | Hneq]; subst.
+  Case "n=l2".
+    destruct (Dominators.member_dec _ l1 (DomDS.st_in _ st) !! l2) 
+      as [Hin12 | Hnotin12]; auto.
+    assert (~ Dominators.member bound l1
+      (DomDS.L.lub bound (DomDS.st_in bound st) !! l2 out)) as Hnotlub12.
+      intro J. apply H0.
+      eapply Dominators.member_eq; eauto.
+    clear J1 J2.
+    destruct (Dominators.member_dec _ l1 out) as [Hinout | Hnotout]; auto.
+    SCase "l1 in out".
+      contradict Hnotlub12. apply Dominators.lub_intro; auto.
+    SCase "l1 notin out".
+      assert (~ Dominators.member _ l1 (transf p (DomDS.st_in bound st) !! p))
+        as Hnotintransf.
+        intro J. apply Hnotout.
+        eapply Dominators.ge_elim in Hout; eauto.
+      unfold transf, transfer in Hnotintransf.
+      assert (l1 <> p /\ ~ Dominators.member _ l1 (DomDS.st_in bound st)!!p) 
+        as J.
+        split; intro J; subst; apply Hnotintransf.
+          apply Dominators.add_member1; auto.
+          apply Dominators.add_member2; auto.
+      clear Hnotintransf.
+      destruct J as [Hneq J].
+      apply Hdom in J; auto.
+      destruct J as [vl [al [J1 J2]]].
+      exists (index p::vl). exists (A_ends (index l2) (index p)::al).
+      split.
+        apply make_predecessors_correct' in Hinpds.
+        change (successors_blocks bs) with (successors (fdef_intro fh bs)) 
+          in Hinpds.
+        apply successors__blockInFdefB in Hinpds.
+        destruct Hinpds as [ps0 [cs0 [tmn0 [J3 J4]]]].
+        constructor; auto.
+          eapply wf_fdef__blockInFdefB__wf_block in J3; eauto.
+          inv J3. inv HwfF.
+          eapply wf_tmn__in_successors in H12; eauto.
+          destruct H12 as [cs1 [ps1 [tmn1 H12]]].
+          eapply blockInFdefB_in_vertexes; eauto.
+
+          inv HwfF.
+          eapply successor_in_arcs; eauto.
+
+          intro J. simpl in J. 
+          destruct J as [J | J]; auto.
+            inv J. auto.
+  Case "n<>l2".
+    rewrite J2 in H0; auto.
+Qed.
+
+Lemma propagate_succ_list_non_sdomination_aux:
+  forall p scs st out,
+  (forall s, In s scs -> In p predecessors!!!s) ->
+  non_sdomination_prop st.(DomDS.st_in _) ->   
+  Dominators.ge _ (transf p st.(DomDS.st_in _)!!p) out ->
+  non_sdomination_prop (DomDS.propagate_succ_list _ st out scs).(DomDS.st_in _).
+Proof.
+  induction scs; simpl; intros; auto.
+    apply IHscs; auto.
+      eapply propagate_succ_non_sdomination; eauto.
+      apply Dominators.ge_trans with (y:=transf p (DomDS.st_in _ st) !! p);
+        auto.
+        eapply EntryDomsOthers.transf_mono; eauto.
+        destruct (@DomDS.propagate_succ_spec _ st out a) as [J1 J2].
+        destruct (eq_atom_dec a p); subst.
+          apply Dominators.ge_trans with 
+            (y:=Dominators.lub _ (DomDS.st_in _ st) !! p out).
+            apply Dominators.ge_refl; auto.
+            apply Dominators.ge_lub_left.
+          rewrite J2; auto.
+            apply Dominators.ge_refl'.
+Qed.
+
+Lemma propagate_succ_list_non_sdomination:
+  forall p scs st,
+  (forall s, In s scs -> In p predecessors!!!s) ->
+  non_sdomination_prop st.(DomDS.st_in _) ->
+  non_sdomination_prop (DomDS.propagate_succ_list _ st 
+    (transf p st.(DomDS.st_in _)!!p) scs).(DomDS.st_in _).
+Proof.
+  intros.
+  eapply propagate_succ_list_non_sdomination_aux; eauto.
+    apply Dominators.ge_refl'.
+Qed.
+
+Lemma step_non_sdomination:
+  forall st n rem,
+  AtomNodeSet.pick st.(DomDS.st_wrk _) = Some(n, rem) ->
+  non_sdomination_prop st.(DomDS.st_in _) ->
+  non_sdomination_prop (DomDS.propagate_succ_list _ 
+                                 (DomDS.mkstate _ st.(DomDS.st_in _) rem)
+                                 (transf n st.(DomDS.st_in _)!!n)
+                                 ((successors_blocks bs)!!!n)).(DomDS.st_in _).
+Proof.
+  intros st n rem WKL GOOD.
+  destruct st. simpl.
+  apply propagate_succ_list_non_sdomination; auto.
+    apply make_predecessors_correct.
+Qed.
+
+Theorem dom_non_sdomination: forall res, 
+  DomDS.fixpoint _ (successors_blocks bs) transf entrypoints = Some res -> 
+  non_sdomination_prop res.
+Proof.
+  unfold DomDS.fixpoint. intros res PI. pattern res. 
+  eapply (PrimIter.iterate_prop _ _ (DomDS.step _ _ _) 
+    (fun st => non_sdomination_prop st.(DomDS.st_in _))); eauto.
+    intros st GOOD. unfold DomDS.step. 
+    caseEq (AtomNodeSet.pick st.(DomDS.st_wrk _)); auto.
+    intros [n rem] PICK. apply step_non_sdomination; auto. 
+
+    apply start_non_sdomination.
+Qed.
+
+End DomComplete. End DomComplete.
+
+Lemma reachable_successors:
+  forall ifs S M f l0 cs ps tmn l1,
+  uniqFdef f -> wf_fdef ifs S M f ->
+  blockInFdefB (block_intro l0 cs ps tmn) f ->
+  In l1 (successors_terminator tmn) ->
+  reachable f l0 ->
+  reachable f l1.
+Proof.
+  intros ifs S M f l0 cs ps tmn l1 HuniqF HwfF HbInF Hin.
+  unfold reachable. intro Hreach.
+  remember (getEntryBlock f) as R.
+  destruct R; auto.
+  destruct b as [le ? ? ?].
+  destruct Hreach as [vl [al Hreach]].
+  exists (index l0::vl). exists (A_ends (index l1) (index l0)::al).
+  apply DW_step; auto.
+    eapply wf_fdef__wf_tmn in HbInF; eauto.    
+    eapply wf_tmn__in_successors in HbInF; eauto.
+    destruct HbInF as [cs1 [ps1 [tmn1 HbInF]]].
+    eapply blockInFdefB_in_vertexes; eauto.
+
+    eapply successor_in_arcs; eauto.
+Qed.
+
+Module UnreachableDoms. Section UnreachableDoms.
+
+Variable ifs : intrinsic_funs.
+Variable S : system.
+Variable M : module.
+Variable fh : fheader.
+Variable bs : blocks.
+Definition bound := bound_blocks bs.
+Definition predecessors := make_predecessors (successors_blocks bs).
+Definition transf := transfer bound.
+Definition top := Dominators.top bound.
+Definition bot := Dominators.bot bound.
+Definition dt := DomDS.dt bound.
+Variable entry: l.
+Variable entrypoints: list (atom * dt).
+
+Hypothesis wf_entrypoints:
+  predecessors!!!entry = nil /\
+  match bs with
+  | block_intro l0 _ _ _ :: _ => l0 = entry
+  | _ => False 
+  end /\
+  exists v, [(entry, v)] = entrypoints /\ Dominators.eq _ v top.
+
+Hypothesis HwfF: wf_fdef ifs S M (fdef_intro fh bs).
+Hypothesis HuniqF: uniqFdef (fdef_intro fh bs).
+
+Definition unrechable_doms (res: AMap.t dt) : Prop :=
+  forall l0, ~ reachable (fdef_intro fh bs) l0 -> l0 <> entry -> 
+  Dominators.eq _ res!!l0 bot.
+
+Lemma start_unrechable_doms: 
+  unrechable_doms 
+    (DomDS.st_in _ (DomDS.start_state _ (successors_blocks bs) entrypoints)).
+Proof.
+  intros l0 Hunreach Heq.
+  unfold DomDS.start_state. simpl.
+  eapply EntryDomsOthers.dom_nonentry_start_state_in in Heq; eauto.
+Qed.
+
+(** We show that the start state satisfies the invariant, and that
+  the [step] function preserves it. *)
+
+Lemma propagate_succ_unrechable_doms: forall st n out,
+  (~ reachable (fdef_intro fh bs) n -> n <> entry -> Dominators.eq _ out bot) ->
+  unrechable_doms st.(DomDS.st_in _) -> 
+  unrechable_doms (DomDS.propagate_succ _ st out n).(DomDS.st_in _).
+Proof.
+  unfold unrechable_doms.
+  intros. 
+  destruct (@DomDS.propagate_succ_spec _ st out n) as [J1 J2].
+  assert (H':=H1). 
+  apply H0 in H1; auto.
+  destruct (eq_atom_dec n l0); subst.
+    apply H in H'; auto.
+    apply Dominators.eq_trans with 
+      (y:=DomDS.L.lub bound (DomDS.st_in bound st) !! l0 out); auto.
+    apply Dominators.eq_trans with (y:=DomDS.L.lub _ bot bot); auto.
+       apply Dominators.lub_compat_eq; auto.
+       apply Dominators.eq_sym. apply Dominators.lub_refl.
+
+    rewrite J2; auto.
+Qed.
+
+Lemma propagate_succ_list_unrechable_doms:
+  forall scs st out,
+  (forall s, In s scs ->
+             ~ reachable (fdef_intro fh bs) s -> s <> entry ->
+             Dominators.eq _ out bot) ->
+  unrechable_doms st.(DomDS.st_in _) ->   
+  unrechable_doms (DomDS.propagate_succ_list _ st out scs).(DomDS.st_in _).
+Proof.
+  induction scs; simpl; intros; auto.
+    apply IHscs.
+      intros. apply H with (s:=s); auto.
+      apply propagate_succ_unrechable_doms; auto.
+        intros J1 J2. eapply H; eauto.
+Qed.
+
+Lemma step_unrechable_doms:
+  forall st n rem,
+  AtomNodeSet.pick st.(DomDS.st_wrk _) = Some(n, rem) ->
+  unrechable_doms st.(DomDS.st_in _) ->
+  unrechable_doms (DomDS.propagate_succ_list _ 
+                                  (DomDS.mkstate _ st.(DomDS.st_in _) rem)
+                                  (transf n st.(DomDS.st_in _)!!n)
+                                  ((successors_blocks bs)!!!n)).(DomDS.st_in _).
+Proof.
+  intros st n rem WKL GOOD.
+  destruct st. simpl.
+  apply propagate_succ_list_unrechable_doms; auto.
+  intros s Hin Hunreach.
+    destruct (reachable_dec (fdef_intro fh bs) n).
+      assert(exists ps0, exists cs0, exists tmn0, 
+        blockInFdefB (block_intro n ps0 cs0 tmn0) (fdef_intro fh bs) /\
+        In s (successors_terminator tmn0)) as J.
+        apply successors__blockInFdefB; auto.
+      destruct J as [ps0 [cs0 [tmn0 [J1 J2]]]].
+      eapply reachable_successors with (l1:=s) in H; eauto.
+      congruence.
+
+      apply GOOD in H. simpl in H.
+      unfold transf, transfer.
+      intros. 
+      destruct (eq_atom_dec n entry); subst.
+        assert (exists ps0, exists cs0, exists tmn0, 
+          blockInFdefB (block_intro entry ps0 cs0 tmn0) (fdef_intro fh bs) /\
+          In s (successors_terminator tmn0)) as J.
+          apply successors__blockInFdefB; auto.
+        destruct J as [ps0 [cs0 [tmn0 [J1 J2]]]].
+        contradict Hunreach.
+        unfold reachable. inv HwfF. rewrite H8. 
+        destruct block5.
+        destruct wf_entrypoints as [_ [J _]].
+        destruct bs; tinv J.
+        destruct b. subst entry.
+        unfold successors_list in Hin. simpl in Hin. rewrite ATree.gss in Hin.
+        clear H1 J. inv H8.
+        exists (index l0::nil). exists (A_ends (index s) (index l0)::nil).
+        constructor.
+          constructor.
+            eapply entry_in_vertexes; simpl; eauto.          
+          inv H14. inv H11.
+          eapply wf_tmn__in_successors in Hin; eauto.
+          destruct Hin as [cs1 [ps1 [tmn1 Hin]]].
+          eapply blockInFdefB_in_vertexes; eauto.
+
+          eapply successor_in_arcs; eauto.
+      apply Dominators.eq_trans with (y:=Dominators.add _ (Dominators.bot _) n).
+        apply Dominators.add_eq; auto.
+        apply Dominators.add_bot.
+Qed.
+
+Theorem dom_unrechable_doms: forall res, 
+  DomDS.fixpoint _ (successors_blocks bs) transf entrypoints = Some res -> 
+  unrechable_doms res.
+Proof.
+  unfold DomDS.fixpoint. intros res PI. pattern res. 
+  eapply (PrimIter.iterate_prop _ _ (DomDS.step _ _ _) 
+    (fun st => unrechable_doms st.(DomDS.st_in _))); eauto.
+  intros st GOOD. unfold DomDS.step. 
+  caseEq (AtomNodeSet.pick st.(DomDS.st_wrk _)); auto.
+  intros [n rem] PICK. 
+  apply step_unrechable_doms; auto. 
+    apply start_unrechable_doms.
+Qed.
+
+End UnreachableDoms. 
+
+End UnreachableDoms.
+
+Lemma dom_unreachable: forall
+  ifs S M (f : fdef) (l3 : l) (l' : l) ps cs tmn
+  (HwfF : wf_fdef ifs S M f) (HuniqF: uniqFdef f)
+  (HBinF : blockInFdefB (block_intro l3 ps cs tmn) f = true)
+  (Hunreach: ~ reachable f l3)
+  (Hnempty: DomDS.L.bs_contents _ ((dom_analyze f) !! l3) <> nil),
+  DomDS.L.eq _ ((dom_analyze f) !! l3) (DomDS.L.bot _).
+Proof.
+  intros. 
+  assert (HwfF':=HwfF). inv HwfF'.
+  destruct block5. 
+  rename blocks5 into bs.
+  assert (J:=H4). destruct bs; inv J. 
+  apply dom_entrypoint in H4.
+  destruct (id_dec l3 l0); subst.
+    rewrite H4 in Hnempty. congruence.
+   
+    clear H. 
+    unfold dom_analyze in *. 
+    remember (entry_dom (block_intro l0 p c t :: bs)) as R.
+    destruct R as [R Hp].
+    destruct R as [[le start] | ]; tinv Hp.
+    destruct start; tinv Hp.
+    destruct bs_contents; tinv Hp. inv HeqR.
+    remember (DomDS.fixpoint (bound_blocks (block_intro l0 p c t :: bs))
+                  (successors_blocks (block_intro l0 p c t :: bs))
+                  (transfer (bound_blocks (block_intro l0 p c t :: bs)))
+                  ((l0,
+                   {|
+                   DomDS.L.bs_contents := nil;
+                   DomDS.L.bs_bound := bs_bound |}) :: nil)) as R.
+    destruct R.
+      symmetry in HeqR. 
+      eapply UnreachableDoms.dom_unrechable_doms with (entry:=l0) in HeqR; 
+        eauto.
+        split. 
+           remember ((DomComplete.predecessors (block_intro l0 p c t :: bs)) 
+             !!! l0) as R.
+           destruct R; auto.
+           assert (In a (DomComplete.predecessors (block_intro l0 p c t :: bs)) 
+             !!! l0) as Hin. rewrite <- HeqR0. simpl; auto.
+           unfold DomComplete.predecessors in Hin.
+           apply make_predecessors_correct' in Hin.
+           apply successors_blocks__blockInFdefB with (fh:=fheader5) in Hin.
+           destruct Hin as [ps0 [cs0 [tmn0 [J1 J2]]]].
+           eapply getEntryBlock_inv with (l3:=a)(a:=l0) in J2; simpl; eauto.
+           congruence.
+
+        split; auto.
+               exists {| DomDS.L.bs_contents := nil; 
+                         DomDS.L.bs_bound := bs_bound |}.
+               split; auto. simpl. apply set_eq_refl. 
+
+      simpl in Hnempty.
+      destruct (id_dec l0 l3); subst.
+        rewrite AMap.gss in *. simpl in *. congruence.
+        rewrite AMap.gso; auto. rewrite AMap.gso in Hnempty; auto. 
+        rewrite AMap.gi in *; auto. simpl in *. unfold ListSet.empty_set in *. 
+        congruence.
+Qed.
+
+Definition domination (f:fdef) (l1 l2:l) : Prop :=
+match getEntryBlock f with
+| Some (block_intro entry _ _ _) =>
+  let vertexes := vertexes_fdef f in
+  let arcs := arcs_fdef f in
+  forall vl al, 
+    D_walk vertexes arcs (index l2) (index entry) vl al -> 
+    (In (index l1) vl \/ l1 = l2)
+| _ => False
+end.
+
+Definition strict_domination (f:fdef) (l1 l2:l) : Prop :=
+domination f l1 l2 /\ l1 <> l2.
+
+Lemma sdom_is_complete: forall
+  ifs S M (f : fdef) (l3 : l) (l' : l) ps cs tmn ps' cs' tmn'
+  (HwfF : wf_fdef ifs S M f) (HuniqF : uniqFdef f)
+  (HBinF' : blockInFdefB (block_intro l' ps' cs' tmn') f = true)
+  (HBinF : blockInFdefB (block_intro l3 ps cs tmn) f = true)
+  (Hsdom: strict_domination f l' l3)
+  (Hnempty: DomDS.L.bs_contents _ ((dom_analyze f) !! l3) <> nil),
+  In l' (DomDS.L.bs_contents _ ((dom_analyze f) !! l3)).
+Proof.
+  intros. unfold dom_analyze in *. destruct f as [fh bs].
+  remember (entry_dom bs) as R.
+  destruct R as [R Hp].
+  destruct R as [[le start] | ].
+    destruct start; tinv Hp.
+    destruct bs_contents; tinv Hp. 
+    destruct bs; tinv HeqR.
+    destruct b; inv HeqR.
+    remember (DomDS.fixpoint (bound_blocks (block_intro l0 p c t :: bs))
+                  (successors_blocks (block_intro l0 p c t :: bs))
+                  (transfer (bound_blocks (block_intro l0 p c t :: bs)))
+                  ((l0,
+                   {|
+                   DomDS.L.bs_contents := nil;
+                   DomDS.L.bs_bound := bs_bound |}) :: nil)) as R.
+    destruct R.
+      symmetry in HeqR.
+      eapply DomComplete.dom_non_sdomination with (entry:=l0) in HeqR; eauto.
+        Focus.
+        unfold DomComplete.non_sdomination_prop in HeqR.
+        destruct (in_dec eq_atom_dec l'
+          (DomDS.L.bs_contents
+            (bound_fdef (fdef_intro fh (block_intro l0 p c t :: bs))) 
+            t0 !! l3)); auto.
+        assert (vertexes_fdef (fdef_intro fh (block_intro l0 p c t :: bs))
+           (index l')) as J. 
+          apply blockInFdefB_in_vertexes in HBinF'; auto.
+        apply HeqR with (l2:=l3) in J.
+          unfold DomComplete.non_sdomination in J.
+          destruct J as [vl [al [J1 J2]]].
+          unfold strict_domination in Hsdom.
+          destruct Hsdom as [Hdom Hneq].
+          unfold domination in Hdom.
+          simpl in Hdom.
+          apply Hdom in J1.
+          destruct J1; subst; congruence.
+         
+          unfold Dominators.member. 
+          unfold DomComplete.dt. unfold DomComplete.bound.
+          destruct (t0!!l3). simpl in *; auto.
+        Unfocus.
+
+        assert (HwfF':=HwfF). inv HwfF'.
+        split. 
+           remember ((DomComplete.predecessors (block_intro l0 p c t :: bs)) 
+             !!! l0) as R.
+           destruct R; auto.
+           assert (In a (DomComplete.predecessors (block_intro l0 p c t :: bs)) 
+             !!! l0) as Hin. rewrite <- HeqR0. simpl; auto.
+           unfold DomComplete.predecessors in Hin.
+           apply make_predecessors_correct' in Hin.
+           apply successors_blocks__blockInFdefB with (fh:=
+             (fheader_intro fnattrs5 typ_5 id_5
+                (map_list_typ_attributes_id
+                   (fun (typ_ : typ) (attributes_ : attributes) (id_ : id) =>
+                    (typ_, attributes_, id_)) typ_attributes_id_list) varg5)) 
+             in Hin.
+           destruct Hin as [ps0 [cs0 [tmn0 [J1 J2]]]].
+           eapply getEntryBlock_inv with (l3:=a)(a:=l0) in J2; simpl; eauto.
+           congruence.
+
+        split; auto.
+               exists {| DomDS.L.bs_contents := nil; DomDS.L.bs_bound := bs_bound |}.
+               split; auto. simpl. apply set_eq_refl. 
+
+      simpl in Hnempty.
+      destruct (id_dec l0 l3); subst.
+        rewrite AMap.gss in *. simpl in *. auto.
+        rewrite AMap.gso in *; auto. rewrite AMap.gi in *; auto. 
+        simpl in *. auto.
+
+    subst. inv HBinF.
+Qed.
+
+Lemma dom_is_sound : forall
+  ifs S M (f : fdef) (l3 : l) (l' : l) ps cs tmn
+  (HwfF : wf_fdef ifs S M f) (HuniqF : uniqFdef f)
+  (HBinF : blockInFdefB (block_intro l3 ps cs tmn) f = true)
+  (Hin : 
+    In l' (l3::(DomDS.L.bs_contents _ ((dom_analyze f) !! l3)))),
+  domination f l' l3.
+Proof. 
+  unfold domination, strict_domination.
+  intros. destruct f as [fh bs].
+  apply uniqF__uniqBlocks in HuniqF.
+  assert (HwfF':=HwfF).
+  apply wf_fdef__non_entry in HwfF'.
+  remember (getEntryBlock (fdef_intro fh bs)) as R.
+  destruct R; auto. clear HwfF'.
+  destruct b as [l5 ps5 cs5 t5].
+  intros vl al Hreach.
+  generalize dependent ps.
+  generalize dependent cs.
+  generalize dependent tmn.
+  remember (vertexes_fdef (fdef_intro fh bs)) as Vs.
+  remember (arcs_fdef (fdef_intro fh bs)) as As.
+  remember (index l3) as v0.
+  remember (index l5) as v1.
+  generalize dependent bs.
+  generalize dependent l3.
+  generalize dependent l5.
+  induction Hreach; intros; subst.
+    inv Heqv0. symmetry in HeqR.
+    apply dom_entrypoint in HeqR.
+    rewrite HeqR in Hin.
+    simpl in Hin. destruct Hin as [Hin | Hin]; tinv Hin; auto.
+
+    destruct y as [a0].
+    assert (exists ps0, exists cs0, exists tmn0, 
+      blockInFdefB (block_intro a0 ps0 cs0 tmn0) (fdef_intro fh bs) /\
+      In l3 (successors_terminator tmn0)) as J.
+      eapply successors__blockInFdefB; eauto.
+    destruct J as [ps0 [cs0 [tmn0 [HBinF'' Hinsucc]]]].
+    remember ((dom_analyze (fdef_intro fh bs)) !! a0) as R.
+    destruct R as [bs_contents bs_bounds].
+    destruct (id_dec l' l3); subst; auto.
+    left.
+    assert (In l'
+      (a0 :: DomDS.L.bs_contents (bound_fdef (fdef_intro fh bs))
+                (dom_analyze (fdef_intro fh bs)) !! a0)) as J.
+      remember ((dom_analyze (fdef_intro fh bs)) !! l3) as R.
+      destruct R.
+      assert (incl bs_contents0 (a0 :: bs_contents)) as Hinc.
+        eapply dom_successors; eauto.
+      rewrite <- HeqR0. simpl.
+      simpl in Hin. destruct Hin; try congruence.
+      apply Hinc; auto.
+    eapply IHHreach in J; eauto.
+    simpl.
+    destruct J as [J | J]; subst; eauto.
+Qed.
+
+Lemma sdom_is_sound : forall
+  ifs S M (f : fdef) (l3 : l) (l' : l) ps cs tmn
+  (HwfF : wf_fdef ifs S M f) (HuniqF : uniqFdef f) (Hreach : reachable f l3)
+  (HBinF : blockInFdefB (block_intro l3 ps cs tmn) f = true)
+  (Hin : 
+    In l' (DomDS.L.bs_contents _ ((dom_analyze f) !! l3))),
+  strict_domination f l' l3.
+Proof. 
+  intros.
+  eapply dom_is_sound with (l':=l') in HBinF; simpl; eauto.
+  split; auto.
+  destruct (id_dec l' l3); subst; auto.
+  unfold reachable, domination in *.
+  remember (getEntryBlock f) as R.
+  destruct R; try congruence.
+  destruct b.
+  destruct Hreach as [vl [al Hreach]].
+  apply DWalk_to_dpath in Hreach.
+  destruct Hreach as [vl0 [al0 Hp]].
+  destruct (id_dec l3 l0); subst.
+    symmetry in HeqR.
+    apply dom_entrypoint in HeqR.
+    rewrite HeqR in Hin. inv Hin.
+
+    inv Hp; try congruence.
+    destruct y as [a0].
+    assert (exists ps0, exists cs0, exists tmn0, 
+      blockInFdefB (block_intro a0 ps0 cs0 tmn0) f /\
+      In l3 (successors_terminator tmn0)) as J.
+      eapply successors__blockInFdefB; eauto.
+    destruct J as [ps0 [cs0 [tmn0 [HBinF' Hinsucc]]]].
+    remember ((dom_analyze f) !! a0) as R.
+    destruct R as [bs_contents bs_bounds].
+    assert (In l3
+      (a0 :: DomDS.L.bs_contents (bound_fdef f)
+                (dom_analyze f) !! a0)) as J.
+      remember ((dom_analyze f) !! l3) as R.
+      destruct R.
+      assert (incl bs_contents0 (a0 :: bs_contents)) as Hinc.
+        destruct f. apply uniqF__uniqBlocks in HuniqF.
+        eapply dom_successors; eauto.
+      rewrite <- HeqR0. simpl.
+      simpl in Hin. 
+      apply Hinc; auto.
+    eapply dom_is_sound in J; eauto.
+    unfold domination in J.
+    rewrite <- HeqR in J.
+    assert (Hw:=H).
+    apply D_path_isa_walk in Hw.
+    apply J in Hw.
+    destruct Hw as [Hw | Hw]; subst; try congruence.
+    apply H4 in Hw. inv Hw; try congruence.
+Qed.
+
+Lemma sdom_isnt_refl : forall
+  ifs S M (f : fdef) (l3 : l) (l' : l) ps cs tmn
+  (HwfF : wf_fdef ifs S M f) (HuniqF : uniqFdef f) (Hreach : reachable f l3)
+  (HBinF : blockInFdefB (block_intro l3 ps cs tmn) f = true)
+  (Hin : In l' (DomDS.L.bs_contents _ ((dom_analyze f) !! l3))),
+  l' <> l3.
+Proof.
+  intros.
+  eapply sdom_is_sound in Hin; eauto.
+  destruct Hin; auto.
+Qed.
+
+Lemma blockStrictDominates_isnt_refl : forall ifs S M F1 block'
+  (Hin : blockInFdefB block' F1) (HwfF : wf_fdef ifs S M F1) 
+  (HuniqF : uniqFdef F1) (Hreach : isReachableFromEntry F1 block'),
+  ~ blockStrictDominates F1 block' block'.
+Proof.
+  intros. destruct block'.
+  unfold blockStrictDominates. intro J.
+  remember ((dom_analyze F1) !! l0) as R.
+  destruct R.
+  simpl in Hreach.
+  eapply sdom_isnt_refl in Hreach; eauto.
+  rewrite <- HeqR. simpl. auto.
+Qed.
+
+Lemma dom_tran: forall (f:fdef) (l1 l2 l3:l),
+  domination f l1 l2 -> domination f l2 l3 -> domination f l1 l3.
+Proof.
+  unfold domination.
+  intros.
+  destruct (getEntryBlock f); tinv H.
+  destruct b.
+  intros vl al Hw.
+  destruct (id_dec l1 l3); auto.
+  left.
+  assert (Hw':=Hw).
+  apply H0 in Hw'.
+  destruct Hw' as [Hw' | Hw']; subst.
+    apply DW_extract with (x:=index l2) in Hw; simpl; auto.
+    destruct Hw as [al' Hw].
+    assert (Hw'':=Hw).
+    apply H in Hw''.
+    destruct Hw'' as [Hw'' | Hw'']; subst; auto.
+    destruct (id_dec l1 l2); subst; auto.
+    apply V_extract_spec in Hw''; try congruence.
+    simpl in Hw''. destruct Hw'' as [Hw'' | Hw'']; congruence.
+
+    assert (Hw'':=Hw).
+    apply H in Hw''.
+    destruct Hw'' as [Hw'' | Hw'']; subst; congruence.
+Qed.     
+
+Lemma dom_acyclic: forall ifs S M (f:fdef) (l1 l2:l) 
+  (HwfF:wf_fdef ifs S M f) (HuniqF : uniqFdef f),
+  reachable f l2 ->
+  strict_domination f l1 l2 -> ~ domination f l2 l1.
+Proof.
+  unfold reachable, strict_domination, domination. 
+  intros. assert (HwfF':=HwfF). 
+  apply wf_fdef__non_entry in HwfF'.
+  remember (getEntryBlock f) as R.
+  destruct R; auto. clear HwfF'.
+  destruct b.
+  destruct H as [vl [al Hw]].
+  apply DWalk_to_dpath in Hw.
+  destruct Hw as [vl0 [al0 Hp]].
+  assert (Hw:=Hp).
+  apply D_path_isa_walk in Hw.
+  destruct H0 as [J1 J2].
+  assert (Hw':=Hw).
+  apply J1 in Hw'.
+  destruct Hw' as [Hw' | Hw']; subst; try congruence.
+  intros J.
+  apply DW_extract with (x:=index l1) in Hw; simpl; auto.
+  destruct Hw as [al' Hw].
+  assert (Hw'':=Hw).
+  apply J in Hw''.
+  destruct Hw'' as [Hw'' | Hw'']; subst; auto.
+  apply V_extract_spec' in Hw''; try congruence.
+  inv Hp. 
+    inv Hw'.
+
+    simpl in Hw''. 
+    destruct Hw'' as [Hw'' | Hw'']; subst; try congruence.
+    apply H4 in Hw''. inv Hw''.
+    destruct y as [a0].
+    assert (exists ps0, exists cs0, exists tmn0, 
+      blockInFdefB (block_intro a0 ps0 cs0 tmn0) f /\
+      In l0 (successors_terminator tmn0)) as J'.
+      eapply successors__blockInFdefB; eauto.
+    destruct J' as [ps0 [cs0 [tmn0 [HBinF' Hinsucc]]]].
+    symmetry in HeqR. destruct f.
+    eapply getEntryBlock_inv in HeqR; eauto.    
+Qed.
+
+Lemma sdom_reachable : forall f l1 l2,
+  reachable f l2 -> strict_domination f l1 l2 -> reachable f l1.
+Proof.
+  unfold reachable, strict_domination, domination.
+  intros.
+  destruct H0 as [J1 J2].
+  destruct (getEntryBlock f); try congruence.
+  destruct b.
+  destruct H as [vl [al H]].
+  assert (H':=H).
+  apply J1 in H'.
+  assert (In (index l1) vl) as Hin.
+    destruct H' as [H' | H']; subst; try congruence.
+  apply DW_extract with (x:=index l1) in H; simpl; auto.
+  destruct H as [al' H].
+  exists (V_extract (index l1) (index l2 :: vl)). exists al'.
+  auto.
+Qed.
+   
+Lemma dom_reachable : forall f l1 l2,
+  reachable f l2 -> domination f l1 l2 -> reachable f l1.
+Proof.
+  intros.
+  destruct (id_dec l1 l2); subst; auto.
+  eapply sdom_reachable; eauto. split; auto.
+Qed.
+
+Lemma sdom_dec : forall f l1 l2,
+  strict_domination f l1 l2 \/ ~ strict_domination f l1 l2.
+Proof. intros. tauto. Qed. (* classic logic *)
+
+Lemma everything_dominates_unreachable_blocks : 
+  forall f l1 l2 (Hreach: ~ reachable f l2) 
+  (Hentry: getEntryBlock f <> None),
+  domination f l1 l2.
+Proof.
+  unfold reachable, domination.
+  intros. 
+  destruct (getEntryBlock f); try congruence.
+  destruct b.
+  intros.
+  contradict Hreach. eauto.
+Qed.  
+
+Lemma sdom_tran1: forall ifs S M (f:fdef) (l1 l2 l3:l) (HwfF:wf_fdef ifs S M f)
+  (HuniqF: uniqFdef f) (Hreach: reachable f l2),
+  strict_domination f l1 l2 -> domination f l2 l3 -> strict_domination f l1 l3.
+Proof.
+  intros.
+  destruct (id_dec l1 l3); subst.
+    eapply dom_acyclic in H; eauto.
+    contradict H; auto.
+
+    destruct H.
+    split; eauto using dom_tran.
+Qed.     
+
+Lemma sdom_tran2: forall ifs S M (f:fdef) (l1 l2 l3:l) (HwfF:wf_fdef ifs S M f)
+  (HuniqF: uniqFdef f) (Hreach: reachable f l3),
+  domination f l1 l2 -> strict_domination f l2 l3 -> strict_domination f l1 l3.
+Proof.
+  intros.
+  destruct (id_dec l1 l3); subst.
+    eapply dom_acyclic in H0; eauto.
+    contradict H0; auto.
+
+    destruct H0.
+    split; eauto using dom_tran.
+Qed.     
+
+Lemma sdom_tran: forall ifs S M (f:fdef) (l1 l2 l3:l) (HwfF:wf_fdef ifs S M f)
+  (HuniqF: uniqFdef f) (Hreach: reachable f l2),
+  strict_domination f l1 l2 -> strict_domination f l2 l3 -> 
+  strict_domination f l1 l3.
+Proof.
+  intros. destruct H0. eapply sdom_tran1; eauto.
+Qed.
+
+Lemma tauto_helper : forall A B:Prop,
+  A -> ~ (B /\ A) -> ~ B.
+Proof. tauto. Qed.
+
+Import Classical_Pred_Type.
+
+Lemma sdom_ordered : forall f l1 l2 l3
+  (Hneq: l1 <> l2) (Hreach: reachable f l3)
+  (Hsdom: strict_domination f l1 l3)
+  (Hsdom': strict_domination f l2 l3),
+  strict_domination f l1 l2 \/ strict_domination f l2 l1.
+Proof.
+  intros.
+  destruct (sdom_dec f l1 l2); auto.
+  destruct (sdom_dec f l2 l1); auto.
+  contradict Hsdom'. intro Hsdom'.
+  unfold strict_domination in *. 
+  destruct Hsdom as [Hdom Hneq1].
+  destruct Hsdom' as [Hdom' Hneq2].
+  unfold domination, reachable in *.
+  destruct (getEntryBlock f); auto.
+  destruct b. 
+  destruct Hreach as [vl [al Hreach]].
+  assert (Hw:=Hreach).  
+  apply Hdom in Hw.
+  destruct Hw as [Hin | Heq]; try congruence.
+  assert (Hw:=Hreach).  
+  apply Hdom' in Hw.
+  destruct Hw as [Hin' | Heq]; try congruence.
+
+  (* on Hw, we need to figuire the closest one to l3 in l1 and l2,
+     suppose l1 is, then we split hw at l1, so l2 cannot be in the part 
+     from l3 to l1.
+  *)
+  assert (Hw:=Hreach).  
+  assert (vl <> V_nil) as Hnqnil.
+    destruct vl; auto.
+      intro J. inv J.
+  apply DW_cut with (x:=index l1) (w:=index l2) in Hw; try congruence; 
+    simpl; auto.
+  destruct Hw as [al1 [al2 [vl1 [vl2 
+    [[J1 [J2 [J3 [J4 J5]]]]|[J1 [J2 [J3 [J4 J5]]]]]]]]]; subst.
+  Case "1".
+  assert (exists vl:V_list, exists al:A_list,
+    D_walk (vertexes_fdef f) (arcs_fdef f) (index l1) (index l0) vl al /\
+    ~ In (index l2) vl) as J.
+    clear - Hneq H0.
+    apply tauto_helper in H0; auto.
+    apply not_all_ex_not in H0. (* can we remove the classic lemma? *)
+    destruct H0 as [vl H0].
+    apply not_all_ex_not in H0.
+    destruct H0 as [al H0].
+    exists vl. exists al.
+    tauto.
+  destruct J as [vl1' [al1' [J1' J2']]].
+
+  assert ((D_walk (vertexes_fdef f) (arcs_fdef f) (index l3) (index l0) 
+    (vl1++vl1') (al1++al1') * ~ In (index l2) (vl1++vl1'))%type) as J.
+    split.
+      eapply DWalk_append; eauto.
+
+      clear - J2' J5.
+      intro J. apply in_app_or in J.
+      simpl in *.
+      destruct J as [J | J]; auto.
+  destruct J as [J3 J4].
+  apply Hdom' in J3.
+  destruct J3 as [Hin'' | Heq]; try congruence.
+
+  Case "2".
+  assert (exists vl:V_list, exists al:A_list,
+    D_walk (vertexes_fdef f) (arcs_fdef f) (index l2) (index l0) vl al /\
+    ~ In (index l1) vl) as J.
+    clear - Hneq H.
+    apply tauto_helper in H; auto.
+    apply not_all_ex_not in H.
+    destruct H as [vl H].
+    apply not_all_ex_not in H.
+    destruct H as [al H].
+    exists vl. exists al.
+    tauto.
+  destruct J as [vl2' [al2' [J1' J2']]].
+
+  assert ((D_walk (vertexes_fdef f) (arcs_fdef f) (index l3) (index l0) 
+    (vl1++vl2') (al1++al2') * ~ In (index l1) (vl1++vl2'))%type) as J.
+    split.
+      eapply DWalk_append; eauto.
+
+      clear - J2' J5.
+      intro J. apply in_app_or in J.
+      simpl in *.
+      destruct J as [J | J]; auto.
+  destruct J as [J3 J4].
+  apply Hdom in J3.
+  destruct J3 as [Hin'' | Heq]; try congruence.
+Qed.
+
+Lemma adom_acyclic: forall l1 l2 ps1 cs1 tmn1 ps2 cs2 tmn2 ifs S M F,
+  wf_fdef ifs S M F -> uniqFdef F ->
+  reachable F l2 ->
+  blockInFdefB (block_intro l1 ps1 cs1 tmn1) F = true ->
+  blockInFdefB (block_intro l2 ps2 cs2 tmn2) F = true ->
+  In l1 (DomDS.L.bs_contents (bound_fdef F) ((dom_analyze F) !! l2)) ->
+  In l2 (DomDS.L.bs_contents (bound_fdef F) ((dom_analyze F) !! l1)) ->
+  l1 <> l2 ->
+  False.
+Proof.
+  intros. 
+  assert (strict_domination F l1 l2) as Hdom12.
+    eapply sdom_is_sound; eauto.
+  assert (strict_domination F l2 l1) as Hdom21.
+    eapply sdom_is_sound; eauto.
+      apply sdom_reachable in Hdom12; auto.
+  eapply dom_acyclic in Hdom12; eauto.
+  apply Hdom12. destruct Hdom21; auto.
+Qed.
+
+Lemma blockStrictDominates_trans : forall ifs S M f b1 b2 b3
+  (HwfF: wf_fdef ifs S M f) (HuniqF: uniqFdef f)
+  (HBinF1: blockInFdefB b1 f)
+  (HBinF2: blockInFdefB b2 f)
+  (HBinF3: blockInFdefB b3 f)
+  (H1 : blockStrictDominates f b1 b2)
+  (H2 : blockStrictDominates f b2 b3),
+  blockStrictDominates f b1 b3.
+Proof.
+  unfold blockStrictDominates.
+  intros. destruct b1, b2, b3.
+  remember (Maps.AMap.get l1 (dom_analyze f)) as R1.
+  remember (Maps.AMap.get l2 (dom_analyze f)) as R2.
+  destruct R1. destruct R2.
+  destruct (reachable_dec f l2).
+    assert (strict_domination f l1 l2) as Hsdom23.
+      eapply sdom_is_sound; eauto.
+        rewrite <- HeqR2. simpl. auto.
+    assert (reachable f l1) as Hreach1.
+      apply sdom_reachable in Hsdom23; auto.
+    assert (strict_domination f l0 l1) as Hsdom12.
+      eapply sdom_is_sound; eauto.
+        rewrite <- HeqR1. simpl. auto.
+    assert (strict_domination f l0 l2) as Hsdom13.
+      eapply sdom_tran with (l2:=l1); eauto.
+    eapply sdom_is_complete in Hsdom13; eauto.
+      rewrite <- HeqR2 in Hsdom13. simpl in *. auto.
+
+      rewrite <- HeqR2. simpl. 
+      destruct bs_contents0; auto.
+        intro J. inv J.
+    
+    eapply dom_unreachable in H; eauto. 
+      rewrite <- HeqR2 in H. simpl in H.
+      destruct H. apply H0.
+      apply blockInFdefB_in_vertexes in HBinF1.
+      unfold vertexes_fdef in HBinF1. auto.
+
+      rewrite <- HeqR2. simpl. intro J. subst. inv H2.
+Qed.
+
+Lemma blockDominates_trans : forall ifs S M f b1 b2 b3
+  (HwfF: wf_fdef ifs S M f) (HuniqF: uniqFdef f)
+  (HBinF1: blockInFdefB b1 f)
+  (HBinF2: blockInFdefB b2 f)
+  (HBinF3: blockInFdefB b3 f)
+  (H1 : blockDominates f b1 b2)
+  (H2 : blockDominates f b2 b3),
+  blockDominates f b1 b3.
+Proof.
+  unfold blockDominates.
+  intros. destruct b1, b2, b3.
+  remember (Maps.AMap.get l1 (dom_analyze f)) as R1.
+  remember (Maps.AMap.get l2 (dom_analyze f)) as R2.
+  destruct R1. destruct R2.
+  destruct (l_dec l0 l2); auto.
+  destruct H2 as [H2 | H2]; subst; auto.
+  Case "l1 in sdom(l2)".
+    left.
+    assert (domination f l1 l2) as Hdom23.
+      eapply dom_is_sound; eauto.
+        rewrite <- HeqR2. simpl. auto.
+    destruct H1 as [H1 | H1]; subst.
+    SCase "l0 in sdom(l1)".
+      assert (domination f l0 l1) as Hdom12.
+        eapply dom_is_sound; eauto.
+          rewrite <- HeqR1. simpl. auto.
+      assert (strict_domination f l0 l2) as Hsdom13.
+        split; auto.
+          eapply dom_tran; eauto.
+      eapply sdom_is_complete in Hsdom13; eauto.
+        rewrite <- HeqR2 in Hsdom13. simpl in *. auto.
+
+        rewrite <- HeqR2. simpl. 
+        destruct bs_contents0; auto.
+          intro J. inv J.
+
+    SCase "l0=l1".
+      assert (strict_domination f l1 l2) as Hsdom12.
+        split; auto.
+      eapply sdom_is_complete in Hsdom12; eauto.
+        rewrite <- HeqR2. simpl. 
+        destruct bs_contents0; auto.
+          intro J. inv J.
+
+  Case "l1=l2".
+    rewrite <- HeqR2 in HeqR1. inv HeqR1; auto.
+Qed.
+
+Module AnotherDominators.
+
+Definition domination (f:fdef) (l1 l2:l) : Prop :=
+match getEntryBlock f with
+| Some (block_intro entry _ _ _) =>
+  let vertexes := vertexes_fdef f in
+  let arcs := arcs_fdef f in
+  forall vl al, 
+    D_walk vertexes arcs (index l2) (index entry) vl al -> 
+    (In (index l1) vl \/ l1 = l2)
+| _ => False
+end.
+
+Definition strict_domination (f:fdef) (l1 l2:l) : Prop :=
+match getEntryBlock f with
+| Some (block_intro entry _ _ _) =>
+  let vertexes := vertexes_fdef f in
+  let arcs := arcs_fdef f in
+  forall vl al, 
+    D_walk vertexes arcs (index l2) (index entry) vl al -> 
+    (In (index l1) vl /\ l1 <> l2)
+| _ => False
+end.
+
+Lemma sdom_is_complete: forall
+  ifs S M (f : fdef) (l3 : l) (l' : l) ps cs tmn ps' cs' tmn'
+  (HwfF : wf_fdef ifs S M f) (HuniqF: uniqFdef f)
+  (HBinF' : blockInFdefB (block_intro l' ps' cs' tmn') f = true)
+  (HBinF : blockInFdefB (block_intro l3 ps cs tmn) f = true)
+  (Hsdom: strict_domination f l' l3)
+  (Hnempty: DomDS.L.bs_contents _ ((dom_analyze f) !! l3) <> nil),
+  In l' (DomDS.L.bs_contents _ ((dom_analyze f) !! l3)).
+Proof.
+  intros. unfold dom_analyze in *. destruct f as [fh bs].
+  remember (entry_dom bs) as R.
+  destruct R as [R Hp].
+  destruct R as [[le start] | ].
+    destruct start; tinv Hp.
+    destruct bs_contents; tinv Hp. 
+    destruct bs; tinv HeqR.
+    destruct b; inv HeqR.
+    remember (DomDS.fixpoint (bound_blocks (block_intro l0 p c t :: bs))
+                  (successors_blocks (block_intro l0 p c t :: bs))
+                  (transfer (bound_blocks (block_intro l0 p c t :: bs)))
+                  ((l0,
+                   {|
+                   DomDS.L.bs_contents := nil;
+                   DomDS.L.bs_bound := bs_bound |}) :: nil)) as R.
+    destruct R.
+      symmetry in HeqR.
+      eapply DomComplete.dom_non_sdomination with (entry:=l0) in HeqR; eauto.
+        Focus.
+        unfold DomComplete.non_sdomination_prop in HeqR.
+        destruct (in_dec eq_atom_dec l'
+          (DomDS.L.bs_contents
+            (bound_fdef (fdef_intro fh (block_intro l0 p c t :: bs))) 
+            t0 !! l3)); auto.
+        assert (vertexes_fdef (fdef_intro fh (block_intro l0 p c t :: bs))
+           (index l')) as J. 
+          apply blockInFdefB_in_vertexes in HBinF'; auto.
+        apply HeqR with (l2:=l3) in J.
+          unfold DomComplete.non_sdomination in J.
+          destruct J as [vl [al [J1 J2]]].
+          unfold strict_domination in Hsdom.
+          simpl in Hsdom.
+          apply Hsdom in J1.
+          destruct J1; subst; congruence.
+         
+          unfold Dominators.member. 
+          unfold DomComplete.dt. unfold DomComplete.bound.
+          destruct (t0!!l3). simpl in *; auto.
+        Unfocus.
+
+        assert (HwfF':=HwfF). inv HwfF'.
+        split. 
+           remember ((DomComplete.predecessors (block_intro l0 p c t :: bs)) 
+             !!! l0) as R.
+           destruct R; auto.
+           assert (In a (DomComplete.predecessors (block_intro l0 p c t :: bs)) 
+             !!! l0) as Hin. rewrite <- HeqR0. simpl; auto.
+           unfold DomComplete.predecessors in Hin.
+           apply make_predecessors_correct' in Hin.
+           apply successors_blocks__blockInFdefB with (fh:=
+             (fheader_intro fnattrs5 typ_5 id_5
+                (map_list_typ_attributes_id
+                   (fun (typ_ : typ) (attributes_ : attributes) (id_ : id) =>
+                    (typ_, attributes_, id_)) typ_attributes_id_list) varg5)) 
+             in Hin.
+           destruct Hin as [ps0 [cs0 [tmn0 [J1 J2]]]].
+           eapply getEntryBlock_inv with (l3:=a)(a:=l0) in J2; simpl; eauto.
+           congruence.
+
+        split; auto.
+               exists {| DomDS.L.bs_contents := nil; 
+                         DomDS.L.bs_bound := bs_bound |}.
+               split; auto. simpl. apply set_eq_refl. 
+
+      simpl in Hnempty.
+      destruct (id_dec l0 l3); subst.
+        rewrite AMap.gss in *. simpl in *. auto.
+        rewrite AMap.gso in *; auto. rewrite AMap.gi in *; auto. 
+        simpl in *. auto.
+
+    subst. inv HBinF.
+Qed.
+
+Lemma dom_is_sound : forall
+  ifs S M (f : fdef) (l3 : l) (l' : l) ps cs tmn
+  (HwfF : wf_fdef ifs S M f) (HuniqF : uniqFdef f)
+  (HBinF : blockInFdefB (block_intro l3 ps cs tmn) f = true)
+  (Hin : 
+    In l' (l3::(DomDS.L.bs_contents _ ((dom_analyze f) !! l3)))),
+  domination f l' l3.
+Proof. 
+  unfold domination, strict_domination.
+  intros. destruct f as [fh bs].
+  apply uniqF__uniqBlocks in HuniqF.
+  assert (HwfF':=HwfF).
+  apply wf_fdef__non_entry in HwfF'.
+  remember (getEntryBlock (fdef_intro fh bs)) as R.
+  destruct R; auto. clear HwfF'.
+  destruct b as [l5 ps5 cs5 t5].
+  intros vl al Hreach.
+  generalize dependent ps.
+  generalize dependent cs.
+  generalize dependent tmn.
+  remember (vertexes_fdef (fdef_intro fh bs)) as Vs.
+  remember (arcs_fdef (fdef_intro fh bs)) as As.
+  remember (index l3) as v0.
+  remember (index l5) as v1.
+  generalize dependent bs.
+  generalize dependent l3.
+  generalize dependent l5.
+  induction Hreach; intros; subst.
+    inv Heqv0. symmetry in HeqR.
+    apply dom_entrypoint in HeqR.
+    rewrite HeqR in Hin.
+    simpl in Hin. destruct Hin as [Hin | Hin]; tinv Hin; auto.
+
+    destruct y as [a0].
+    assert (exists ps0, exists cs0, exists tmn0, 
+      blockInFdefB (block_intro a0 ps0 cs0 tmn0) (fdef_intro fh bs) /\
+      In l3 (successors_terminator tmn0)) as J.
+      eapply successors__blockInFdefB; eauto.
+    destruct J as [ps0 [cs0 [tmn0 [HBinF'' Hinsucc]]]].
+    remember ((dom_analyze (fdef_intro fh bs)) !! a0) as R.
+    destruct R as [bs_contents bs_bounds].
+    destruct (id_dec l' l3); subst; auto.
+    left.
+    assert (In l'
+      (a0 :: DomDS.L.bs_contents (bound_fdef (fdef_intro fh bs))
+                (dom_analyze (fdef_intro fh bs)) !! a0)) as J.
+      remember ((dom_analyze (fdef_intro fh bs)) !! l3) as R.
+      destruct R.
+      assert (incl bs_contents0 (a0 :: bs_contents)) as Hinc.
+        eapply dom_successors; eauto.
+      rewrite <- HeqR0. simpl.
+      simpl in Hin. destruct Hin; try congruence.
+      apply Hinc; auto.
+    eapply IHHreach in J; eauto.
+    simpl.
+    destruct J as [J | J]; subst; eauto.
+Qed.
+
+Lemma sdom_is_sound : forall
+  ifs S M (f : fdef) (l3 : l) (l' : l) ps cs tmn
+  (HwfF : wf_fdef ifs S M f) (HuniqF : uniqFdef f)
+  (HBinF : blockInFdefB (block_intro l3 ps cs tmn) f = true)
+  (Hin : 
+    In l' (DomDS.L.bs_contents _ ((dom_analyze f) !! l3))),
+  strict_domination f l' l3.
+Proof. 
+  intros.
+  eapply dom_is_sound with (l':=l') in HBinF; simpl; eauto.
+  unfold strict_domination, domination in *.
+  remember (getEntryBlock f) as R.
+  destruct R; try congruence.
+  destruct b.
+  intros vl al Hreach.
+  assert (Hw':=Hreach).
+  apply DWalk_to_dpath in Hreach.
+  destruct Hreach as [vl0 [al0 Hp]].
+  destruct (id_dec l' l3); subst; auto.
+  Case "l'=l3".
+    destruct (id_dec l3 l0); subst.
+    SCase "l3=l0".
+      symmetry in HeqR.
+      apply dom_entrypoint in HeqR.
+      rewrite HeqR in Hin. inv Hin.
+
+    SCase "l3<>l0".
+      inv Hp; try congruence.
+      destruct y as [a0].
+      assert (exists ps0, exists cs0, exists tmn0, 
+        blockInFdefB (block_intro a0 ps0 cs0 tmn0) f /\
+        In l3 (successors_terminator tmn0)) as J.
+        eapply successors__blockInFdefB; eauto.
+      destruct J as [ps0 [cs0 [tmn0 [HBinF' Hinsucc]]]].
+      remember ((dom_analyze f) !! a0) as R.
+      destruct R as [bs_contents bs_bounds].
+      assert (In l3
+        (a0 :: DomDS.L.bs_contents (bound_fdef f)
+                  (dom_analyze f) !! a0)) as J.
+        remember ((dom_analyze f) !! l3) as R.
+        destruct R.
+        assert (incl bs_contents0 (a0 :: bs_contents)) as Hinc.
+          destruct f. apply uniqF__uniqBlocks in HuniqF.
+          eapply dom_successors; eauto.
+        rewrite <- HeqR0. simpl.
+        simpl in Hin. 
+        apply Hinc; auto.
+      eapply dom_is_sound in J; eauto.
+      unfold domination in J.
+      rewrite <- HeqR in J.
+      assert (Hw:=H).
+      apply D_path_isa_walk in Hw.
+      apply J in Hw.
+      destruct Hw as [Hw | Hw]; subst; try congruence.
+      apply H4 in Hw. inv Hw; try congruence.
+  Case "l'<>l3".
+    apply HBinF in Hw'.
+    split; auto. destruct Hw'; subst; auto. congruence.
+Qed.
+
+Lemma dom_tran: forall (f:fdef) (l1 l2 l3:l),
+  domination f l1 l2 -> domination f l2 l3 -> domination f l1 l3.
+Proof.
+  unfold domination.
+  intros.
+  destruct (getEntryBlock f); tinv H.
+  destruct b.
+  intros vl al Hw.
+  destruct (id_dec l1 l3); auto.
+  left.
+  assert (Hw':=Hw).
+  apply H0 in Hw'.
+  destruct Hw' as [Hw' | Hw']; subst.
+    apply DW_extract with (x:=index l2) in Hw; simpl; auto.
+    destruct Hw as [al' Hw].
+    assert (Hw'':=Hw).
+    apply H in Hw''.
+    destruct Hw'' as [Hw'' | Hw'']; subst; auto.
+    destruct (id_dec l1 l2); subst; auto.
+    apply V_extract_spec in Hw''; try congruence.
+    simpl in Hw''. destruct Hw'' as [Hw'' | Hw'']; congruence.
+
+    assert (Hw'':=Hw).
+    apply H in Hw''.
+    destruct Hw'' as [Hw'' | Hw'']; subst; congruence.
+Qed.     
+
+Lemma dom_acyclic: forall ifs S M (f:fdef) (l1 l2:l) (HwfF:wf_fdef ifs S M f)
+  (HuniqF: uniqFdef f),
+  reachable f l2 ->
+  strict_domination f l1 l2 -> ~ domination f l2 l1.
+Proof.
+  unfold reachable, strict_domination, domination. 
+  intros. assert (HwfF':=HwfF).
+  apply wf_fdef__non_entry in HwfF'.
+  remember (getEntryBlock f) as R.
+  destruct R; auto. clear HwfF'.
+  destruct b.
+  destruct H as [vl [al Hw]].
+  apply DWalk_to_dpath in Hw.
+  destruct Hw as [vl0 [al0 Hp]].
+  assert (Hw:=Hp).
+  apply D_path_isa_walk in Hw.
+  assert (Hw':=Hw).
+  apply H0 in Hw'.
+  destruct Hw' as [J1 J2].
+  intros J.
+  apply DW_extract with (x:=index l1) in Hw; simpl; auto.
+  destruct Hw as [al' Hw].
+  assert (Hw'':=Hw).
+  apply J in Hw''.
+  destruct Hw'' as [Hw'' | Hw'']; subst; auto.
+  apply V_extract_spec' in Hw''; try congruence.
+  inv Hp. 
+    inv Hw''.
+
+    simpl in Hw''. 
+    destruct Hw'' as [Hw'' | Hw'']; subst; try congruence.
+    apply H5 in Hw''. inv Hw''.
+    destruct y as [a0].
+    assert (exists ps0, exists cs0, exists tmn0, 
+      blockInFdefB (block_intro a0 ps0 cs0 tmn0) f /\
+      In l0 (successors_terminator tmn0)) as J'.
+      eapply successors__blockInFdefB; eauto.
+    destruct J' as [ps0 [cs0 [tmn0 [HBinF' Hinsucc]]]].
+    symmetry in HeqR. destruct f.
+    eapply getEntryBlock_inv in HeqR; eauto.    
+Qed.
+
+Lemma sdom_reachable : forall f l1 l2,
+  reachable f l2 -> strict_domination f l1 l2 -> reachable f l1.
+Proof.
+  unfold reachable, strict_domination.
+  intros.
+  destruct (getEntryBlock f); try congruence.
+  destruct b.
+  destruct H as [vl [al H]].
+  assert (H':=H).
+  apply H0 in H'. destruct H' as [J1 J2].
+  apply DW_extract with (x:=index l1) in H; simpl; auto.
+  destruct H as [al' H].
+  exists (V_extract (index l1) (index l2 :: vl)). exists al'.
+  auto.
+Qed.
+   
+Lemma dom_reachable : forall f l1 l2,
+  reachable f l2 -> domination f l1 l2 -> reachable f l1.
+Proof.
+  unfold reachable, domination.
+  intros.
+  destruct (getEntryBlock f); try congruence.
+  destruct b.
+  destruct H as [vl [al H]].
+  assert (H':=H).
+  apply H0 in H'.
+  apply DW_extract with (x:=index l1) in H; simpl; auto.
+    destruct H as [al' H].
+    exists (V_extract (index l1) (index l2 :: vl)). exists al'. auto.
+
+    destruct H' as [H' | H']; subst; auto.
+Qed.
+
+Lemma everything_dominates_unreachable_blocks : 
+  forall f l1 l2 (Hreach: ~ reachable f l2) 
+  (Hentry: getEntryBlock f <> None),
+  domination f l1 l2.
+Proof.
+  unfold reachable, domination.
+  intros. 
+  destruct (getEntryBlock f); try congruence.
+  destruct b.
+  intros.
+  contradict Hreach. eauto.
+Qed.  
+
+Lemma everything_sdominates_unreachable_blocks : 
+  forall f l1 l2 (Hreach: ~ reachable f l2) 
+  (Hentry: getEntryBlock f <> None),
+  strict_domination f l1 l2.
+Proof.
+  unfold reachable, strict_domination.
+  intros. 
+  destruct (getEntryBlock f); try congruence.
+  destruct b.
+  intros.
+  contradict Hreach. eauto.
+Qed.  
+
+Lemma sdom_dom: forall f l1 l2,
+  strict_domination f l1 l2 -> domination f l1 l2. 
+Proof.
+  unfold strict_domination, domination.
+  intros. 
+  destruct (getEntryBlock f); try congruence.
+  destruct b. intros. apply H in H0. destruct H0; auto.
+Qed.  
+
+Lemma dom_sdom: forall f l1 l2,
+  domination f l1 l2 -> l1 <> l2 -> strict_domination f l1 l2. 
+Proof.
+  unfold strict_domination, domination.
+  intros. 
+  destruct (getEntryBlock f); try congruence.
+  destruct b. intros. apply H in H1. 
+  destruct H1 as [H1 | H1]; subst; auto. 
+    congruence.
+Qed.  
+
+Lemma sdom_tran1: forall ifs S M (f:fdef) (l1 l2 l3:l) (HwfF:wf_fdef ifs S M f)
+  (HuniqF: uniqFdef f),
+  strict_domination f l1 l2 -> domination f l2 l3 -> strict_domination f l1 l3.
+Proof.
+  intros.
+  destruct (id_dec l1 l3); subst.
+    destruct (@reachable_dec f l3).
+      eapply dom_acyclic in H; eauto.
+        contradict H; auto.
+        apply dom_reachable in H0; auto.   
+
+      apply everything_sdominates_unreachable_blocks; auto.
+        eapply wf_fdef__non_entry; eauto.
+
+    apply sdom_dom in H.
+    apply dom_sdom; eauto using dom_tran.
+Qed.
+
+Lemma sdom_tran2: forall ifs S M (f:fdef) (l1 l2 l3:l) (HwfF:wf_fdef ifs S M f)
+  (HuniqF : uniqFdef f),
+  domination f l1 l2 -> strict_domination f l2 l3 -> strict_domination f l1 l3.
+Proof.
+  intros.
+  destruct (id_dec l1 l3); subst.
+    destruct (@reachable_dec f l3).
+      eapply dom_acyclic in H0; eauto.
+      contradict H0; auto.
+
+      apply everything_sdominates_unreachable_blocks; auto.
+        eapply wf_fdef__non_entry; eauto.
+
+    apply sdom_dom in H0.
+    apply dom_sdom; eauto using dom_tran.
+Qed.     
+
+Lemma sdom_tran: forall ifs S M (f:fdef) (l1 l2 l3:l) (HwfF:wf_fdef ifs S M f)
+  (HuniqF: uniqFdef f),
+  strict_domination f l1 l2 -> strict_domination f l2 l3 -> 
+  strict_domination f l1 l3.
+Proof.
+  intros. apply sdom_dom in H0. eapply sdom_tran1; eauto.
+Qed.     
+
+Import Classical_Pred_Type.
+
+Definition strict_domination' f l1 l2 := domination f l1 l2 /\ l1 <> l2.
+
+Lemma sdom_sdom': forall f l1 l2,
+  strict_domination f l1 l2 -> reachable f l2 -> strict_domination' f l1 l2.
+Proof.
+  intros.
+  split. apply sdom_dom; auto.
+    unfold reachable, strict_domination in *. intros.
+    destruct (getEntryBlock f); tinv H.
+    destruct b.
+    destruct H0 as [vl [al H0]]. 
+    apply H in H0; auto.
+Qed.
+
+Lemma sdom_dec' : forall f l1 l2,
+  strict_domination' f l1 l2 \/ ~ strict_domination' f l1 l2.
+Proof. intros. tauto. Qed. (* classic logic *)
+
+Lemma sdom_ordered' : forall f l1 l2 l3
+  (Hneq: l1 <> l2) (Hreach: reachable f l3)
+  (Hsdom: strict_domination' f l1 l3)
+  (Hsdom': strict_domination' f l2 l3),
+  strict_domination' f l1 l2 \/ strict_domination' f l2 l1.
+Proof.
+  intros.
+  destruct (sdom_dec' f l1 l2); auto.
+  destruct (sdom_dec' f l2 l1); auto.
+  contradict Hsdom'. intro Hsdom'.
+  unfold strict_domination' in *. 
+  destruct Hsdom as [Hdom Hneq1].
+  destruct Hsdom' as [Hdom' Hneq2].
+  unfold domination, reachable in *.
+  destruct (getEntryBlock f); auto.
+  destruct b. 
+  destruct Hreach as [vl [al Hreach]].
+  assert (Hw:=Hreach).  
+  apply Hdom in Hw.
+  destruct Hw as [Hin | Heq]; try congruence.
+  assert (Hw:=Hreach).  
+  apply Hdom' in Hw.
+  destruct Hw as [Hin' | Heq]; try congruence.
+
+  (* on Hw, we need to figuire the closest one to l3 in l1 and l2,
+     suppose l1 is, then we split hw at l1, so l2 cannot be in the part 
+     from l3 to l1.
+  *)
+  assert (Hw:=Hreach).  
+  assert (vl <> V_nil) as Hnqnil.
+    destruct vl; auto.
+      intro J. inv J.
+  apply DW_cut with (x:=index l1) (w:=index l2) in Hw; try congruence; 
+    simpl; auto.
+  destruct Hw as [al1 [al2 [vl1 [vl2 
+    [[J1 [J2 [J3 [J4 J5]]]]|[J1 [J2 [J3 [J4 J5]]]]]]]]]; subst.
+  Case "1".
+  assert (exists vl:V_list, exists al:A_list,
+    D_walk (vertexes_fdef f) (arcs_fdef f) (index l1) (index l0) vl al /\
+    ~ In (index l2) vl) as J.
+    clear - Hneq H0.
+    apply tauto_helper in H0; auto.
+    apply not_all_ex_not in H0. (* can we remove the classic lemma? *)
+    destruct H0 as [vl H0].
+    apply not_all_ex_not in H0.
+    destruct H0 as [al H0].
+    exists vl. exists al.
+    tauto.
+  destruct J as [vl1' [al1' [J1' J2']]].
+
+  assert ((D_walk (vertexes_fdef f) (arcs_fdef f) (index l3) (index l0) 
+    (vl1++vl1') (al1++al1') * ~ In (index l2) (vl1++vl1'))%type) as J.
+    split.
+      eapply DWalk_append; eauto.
+
+      clear - J2' J5.
+      intro J. apply in_app_or in J.
+      simpl in *.
+      destruct J as [J | J]; auto.
+  destruct J as [J3 J4].
+  apply Hdom' in J3.
+  destruct J3 as [Hin'' | Heq]; try congruence.
+
+  Case "2".
+  assert (exists vl:V_list, exists al:A_list,
+    D_walk (vertexes_fdef f) (arcs_fdef f) (index l2) (index l0) vl al /\
+    ~ In (index l1) vl) as J.
+    clear - Hneq H.
+    apply tauto_helper in H; auto.
+    apply not_all_ex_not in H.
+    destruct H as [vl H].
+    apply not_all_ex_not in H.
+    destruct H as [al H].
+    exists vl. exists al.
+    tauto.
+  destruct J as [vl2' [al2' [J1' J2']]].
+
+  assert ((D_walk (vertexes_fdef f) (arcs_fdef f) (index l3) (index l0) 
+    (vl1++vl2') (al1++al2') * ~ In (index l1) (vl1++vl2'))%type) as J.
+    split.
+      eapply DWalk_append; eauto.
+
+      clear - J2' J5.
+      intro J. apply in_app_or in J.
+      simpl in *.
+      destruct J as [J | J]; auto.
+  destruct J as [J3 J4].
+  apply Hdom in J3.
+  destruct J3 as [Hin'' | Heq]; try congruence.
+Qed.
+
+Lemma sdom_ordered : forall f l1 l2 l3
+  (Hneq: l1 <> l2) (Hreach: reachable f l3)
+  (Hsdom: strict_domination f l1 l3)
+  (Hsdom': strict_domination f l2 l3),
+  strict_domination f l1 l2 \/ strict_domination f l2 l1.
+Proof.
+  intros.
+  apply sdom_sdom' in Hsdom; auto.
+  apply sdom_sdom' in Hsdom'; auto.
+  assert (J:=Hsdom').
+  eapply sdom_ordered' in J; eauto.
+  destruct J as [[J1 J2] | [J1 J2]].
+    left. apply dom_sdom; auto.
+    right. apply dom_sdom; auto.
+Qed.
+
+Lemma adom_acyclic: forall l1 l2 ps1 cs1 tmn1 ps2 cs2 tmn2 ifs S M F,
+  wf_fdef ifs S M F -> uniqFdef F ->
+  reachable F l2 ->
+  blockInFdefB (block_intro l1 ps1 cs1 tmn1) F = true ->
+  blockInFdefB (block_intro l2 ps2 cs2 tmn2) F = true ->
+  In l1 (DomDS.L.bs_contents (bound_fdef F) ((dom_analyze F) !! l2)) ->
+  In l2 (DomDS.L.bs_contents (bound_fdef F) ((dom_analyze F) !! l1)) ->
+  l1 <> l2 ->
+  False.
+Proof.
+  intros. 
+  assert (strict_domination F l1 l2) as Hdom12.
+    eapply sdom_is_sound; eauto.
+  assert (strict_domination F l2 l1) as Hdom21.
+    eapply sdom_is_sound; eauto.
+  eapply dom_acyclic in Hdom12; eauto.
+  apply Hdom12. apply sdom_dom; auto.
+Qed.
+
+Lemma blockStrictDominates_trans : forall ifs S M f b1 b2 b3
+  (HwfF: wf_fdef ifs S M f) (HuniqF:uniqFdef f)
+  (HBinF1: blockInFdefB b1 f)
+  (HBinF2: blockInFdefB b2 f)
+  (HBinF3: blockInFdefB b3 f)
+  (H1 : blockStrictDominates f b1 b2)
+  (H2 : blockStrictDominates f b2 b3),
+  blockStrictDominates f b1 b3.
+Proof.
+  unfold blockStrictDominates.
+  intros. destruct b1, b2, b3.
+  remember (Maps.AMap.get l1 (dom_analyze f)) as R1.
+  remember (Maps.AMap.get l2 (dom_analyze f)) as R2.
+  destruct R1. destruct R2.
+  destruct (reachable_dec f l2).
+    assert (strict_domination f l1 l2) as Hsdom23.
+      eapply sdom_is_sound; eauto.
+        rewrite <- HeqR2. simpl. auto.
+    assert (reachable f l1) as Hreach1.
+      apply sdom_reachable in Hsdom23; auto.
+    assert (strict_domination f l0 l1) as Hsdom12.
+      eapply sdom_is_sound; eauto.
+        rewrite <- HeqR1. simpl. auto.
+    assert (strict_domination f l0 l2) as Hsdom13.
+      eapply sdom_tran with (l2:=l1); eauto.
+    eapply sdom_is_complete in Hsdom13; eauto.
+      rewrite <- HeqR2 in Hsdom13. simpl in *. auto.
+
+      rewrite <- HeqR2. simpl. 
+      destruct bs_contents0; auto.
+        intro J. inv J.
+    
+    eapply dom_unreachable in H; eauto. 
+      rewrite <- HeqR2 in H. simpl in H.
+      destruct H. apply H0.
+      apply blockInFdefB_in_vertexes in HBinF1.
+      unfold vertexes_fdef in HBinF1. auto.
+
+      rewrite <- HeqR2. simpl. intro J. subst. inv H2.
+Qed.
+
+Lemma blockDominates_trans : forall ifs S M f b1 b2 b3
+  (HwfF: wf_fdef ifs S M f) (HuniqF:uniqFdef f)
+  (HBinF1: blockInFdefB b1 f)
+  (HBinF2: blockInFdefB b2 f)
+  (HBinF3: blockInFdefB b3 f)
+  (H1 : blockDominates f b1 b2)
+  (H2 : blockDominates f b2 b3),
+  blockDominates f b1 b3.
+Proof.
+  unfold blockDominates.
+  intros. destruct b1, b2, b3.
+  remember (Maps.AMap.get l1 (dom_analyze f)) as R1.
+  remember (Maps.AMap.get l2 (dom_analyze f)) as R2.
+  destruct R1. destruct R2.
+  destruct (l_dec l0 l2); auto.
+  destruct H2 as [H2 | H2]; subst; auto.
+  Case "l1 in sdom(l2)".
+    left.
+    assert (domination f l1 l2) as Hdom23.
+      eapply dom_is_sound; eauto.
+        rewrite <- HeqR2. simpl. auto.
+    destruct H1 as [H1 | H1]; subst.
+    SCase "l0 in sdom(l1)".
+      assert (domination f l0 l1) as Hdom12.
+        eapply dom_is_sound; eauto.
+          rewrite <- HeqR1. simpl. auto.
+      assert (strict_domination f l0 l2) as Hsdom13.
+        apply dom_sdom; auto.
+        eapply dom_tran; eauto.
+      eapply sdom_is_complete in Hsdom13; eauto.
+        rewrite <- HeqR2 in Hsdom13. simpl in *. auto.
+
+        rewrite <- HeqR2. simpl. 
+        destruct bs_contents0; auto.
+          intro J. inv J.
+
+    SCase "l0=l1".
+      assert (strict_domination f l1 l2) as Hsdom12.
+        apply dom_sdom; auto.
+      eapply sdom_is_complete in Hsdom12; eauto.
+        rewrite <- HeqR2. simpl. 
+        destruct bs_contents0; auto.
+          intro J. inv J.
+
+  Case "l1=l2".
+    rewrite <- HeqR2 in HeqR1. inv HeqR1; auto.
+Qed.
+End AnotherDominators.
 
 (********************************************)
 (** * feasible typs *)
@@ -3032,6 +4772,6 @@ Qed.
 (*
 *** Local Variables: ***
 *** coq-prog-name: "coqtop" ***
-*** coq-prog-args: ("-emacs-U" "-I" "~/SVN/sol/vol/src/Vellvm/monads" "-I" "~/SVN/sol/vol/src/Vellvm/ott" "-I" "~/SVN/sol/vol/src/Vellvm/compcert" "-I" "~/SVN/sol/theory/metatheory_8.3" "-I" "~/SVN/sol/vol/src/TV") ***
+*** coq-prog-args: ("-emacs-U" "-I" "~/SVN/sol/vol/src/Vellvm/monads" "-I" "~/SVN/sol/vol/src/Vellvm/ott" "-I" "~/SVN/sol/vol/src/Vellvm/compcert" "-I" "~/SVN/sol/theory/metatheory_8.3" "-I" "~/SVN/sol/vol/src/TV" "-impredicative-set") ***
 *** End: ***
  *)
