src/TV/sub_tv_dec.v
@@ -36,7 +36,7 @@ Proof.
       right. intro J. destruct J as [l EQ].
       inversion EQ.
 
-      destruct (@X a a0); subst.
+      destruct (@H a a0); subst.
         destruct (@IHl1 l2).
           left. destruct p as [l EQ]; subst.
           exists l. auto.
@@ -53,6 +53,6 @@ Qed.
 (*
 *** Local Variables: ***
 *** coq-prog-name: "coqtop" ***
-*** coq-prog-args: ("-emacs-U" "-I" "~/SVN/sol/vol/src/Vellvm/monads" "-I" "~/SVN/sol/vol/src/Vellvm/ott" "-I" "~/SVN/sol/vol/src/Vellvm/compcert" "-I" "~/SVN/sol/theory/metatheory_8.3") ***
+*** coq-prog-args: ("-emacs-U" "-I" "~/SVN/sol/vol/src/Vellvm/monads" "-I" "~/SVN/sol/vol/src/Vellvm/ott" "-I" "~/SVN/sol/vol/src/Vellvm/compcert" "-I" "~/SVN/sol/theory/metatheory_8.3" "-impredicative-set") ***
 *** End: ***
  *)
